Update Higher_Proj_Space_Rank_Axioms_To_Higher_Proj_Space_Axioms.thy

Space/Higher_Proj_Space_Rank_Axioms_To_Higher_Proj_Space_Axioms.thy
@@ -1,5 +1,5 @@
 theory Higher_Proj_Space_Rank_Axioms_To_Higher_Proj_Space_Axioms
-  imports Main Higher_Projective_Space_Rank_Axioms
+  imports Main Higher_Projective_Space_Rank_Axioms Matroid_Rank_Properties
 begin
 
 (*
@@ -44,7 +44,17 @@ definition snd :: "lines \<Rightarrow> points" where
 (* Next, we define an incidence relation between points and lines *)
 
 definition incid :: "points \<Rightarrow> lines \<Rightarrow> bool" where
-"incid P l \<equiv> rk {fst l, snd l, P} = 2"
+"incid P l \<equiv> rk {fst l, snd l, P} \<le> 2"
+
+lemma incid_rk :
+  assumes "incid P l"
+  shows "rk {fst l, snd l, P} = 2"
+proof-
+  have "rk {fst l, snd l, P} \<ge> 2"
+    by (metis (mono_tags, lifting) Higher_Proj_Space_Rank_Axioms_To_Higher_Proj_Space_Axioms.fst_def Higher_Proj_Space_Rank_Axioms_To_Higher_Proj_Space_Axioms.snd_def Rep_lines Un_insert_left Un_upper1 insert_is_Un matroid_ax_2 mem_Collect_eq rk_couple)
+  thus "rk {fst l, snd l, P} = 2"
+    using assms incid_def by auto
+qed
 
 (* Then we prove that the higher projective space axioms are satisfied *)
 
@@ -61,31 +71,73 @@ proof-
 qed
   
 lemma ax1_existence : "\<forall>P Q.\<exists>l. (incid P l) \<and> (incid Q l)"
-proof (rule allI, rule allI)
+proof (rule allI)+
   fix P Q
   have f1:"incid P (Abs_lines (line P Q)) \<and> incid Q (Abs_lines (line P Q))" if "P \<noteq> Q"
-    by (smt Abs_lines_inverse Higher_Proj_Space_Rank_Axioms_To_Higher_Proj_Space_Axioms.fst_def Higher_Proj_Space_Rank_Axioms_To_Higher_Proj_Space_Axioms.snd_def fst_pt.simps incid_def insert_commute mem_Collect_eq rk_triple_rep snd_pt.simps that)
+    by (smt Abs_lines_inverse Higher_Proj_Space_Rank_Axioms_To_Higher_Proj_Space_Axioms.fst_def Higher_Proj_Space_Rank_Axioms_To_Higher_Proj_Space_Axioms.snd_def fst_pt.simps incid_def insert_commute mem_Collect_eq order_refl rk_triple_rep snd_pt.simps that)
   define l where "l = Abs_lines (line P (@ R. R \<noteq> P))"
   have f2:"incid P l \<and> incid Q l" if "P = Q"
-    by (smt Abs_lines_induct Abs_lines_inverse Higher_Proj_Space_Rank_Axioms_To_Higher_Proj_Space_Axioms.fst_def Higher_Proj_Space_Rank_Axioms_To_Higher_Proj_Space_Axioms.snd_def fst_pt.simps incid_def insert_commute l_def mem_Collect_eq rk_triple_rep snd_pt.simps some_eq_ex that)
+    by (smt Abs_lines_induct Abs_lines_inverse Higher_Proj_Space_Rank_Axioms_To_Higher_Proj_Space_Axioms.fst_def fst_pt.simps incid_def insert_absorb2 insert_commute l_def matroid_ax_2 mem_Collect_eq rk_triple_rep snd_pt.simps some_eq_ex subset_insertI that)
   from f1 and f2 show "\<exists>l. incid P l \<and> incid Q l" by blast
 qed
 
 definition line_eq :: "lines \<Rightarrow> lines \<Rightarrow> bool" where
-"line_eq k l \<equiv> rk {fst k, snd k, fst l, snd l} = 2"
+"line_eq k l \<equiv> rk {fst k, snd k, fst l, snd l} \<le> 2"
+
+lemma line_eq_rk :
+  assumes "line_eq k l"
+  shows "rk {fst k, snd k, fst l, snd l} = 2"
+proof-
+  have f1:"rk {fst k, snd k, fst l, snd l} \<le> 2"
+    using assms line_eq_def by auto
+  have "fst k \<noteq> snd k \<and> fst l \<noteq> snd l"
+    using Higher_Proj_Space_Rank_Axioms_To_Higher_Proj_Space_Axioms.fst_def Higher_Proj_Space_Rank_Axioms_To_Higher_Proj_Space_Axioms.snd_def Rep_lines by auto
+  then have f2:"rk {fst k, snd k, fst l, snd l} \<ge> 2"
+    by (meson matroid_ax_2 order.trans rk_ax_couple subset_insertI)
+  from f1 and f2 show "rk {fst k, snd k, fst l, snd l} = 2"
+    using antisym_conv by auto
+qed
 
 lemma line_eq_refl : "line_eq l l"
-  by (metis (mono_tags, lifting) Higher_Proj_Space_Rank_Axioms_To_Higher_Proj_Space_Axioms.fst_def Higher_Proj_Space_Rank_Axioms_To_Higher_Proj_Space_Axioms.snd_def Rep_lines insert_absorb2 insert_commute line_eq_def mem_Collect_eq rk_triple_rep)
+  by (smt Higher_Proj_Space_Rank_Axioms_To_Higher_Proj_Space_Axioms.fst_def Higher_Proj_Space_Rank_Axioms_To_Higher_Proj_Space_Axioms.snd_def Rep_lines eq_iff insert_absorb2 insert_commute line_eq_def mem_Collect_eq rk_triple_rep)
 
 lemma line_eq_sym : "line_eq k l = line_eq l k"
   by (simp add: insert_commute line_eq_def)
 
 lemma line_eq_trans : "line_eq k l \<longrightarrow> line_eq l m \<longrightarrow> line_eq k m"
-
+proof(rule impI)+
+  assume "line_eq k l" and "line_eq l m"
+  have "{fst l, snd l} \<subseteq> {fst k, snd k, fst l, snd l} \<inter> {fst l, snd l, fst m, snd m}" by auto
+  then have "rk {fst k, snd k, fst l, snd l, fst m, snd m} + rk {fst l, snd l} \<le> 
+    rk {fst k, snd k, fst l, snd l} + rk {fst l, snd l, fst m, snd m}" using matroid_ax_3_alt
+    by (smt Un_insert_left le_infE sup.absorb_iff2)
+  then have "rk {fst k, snd k, fst l, snd l, fst m, snd m} \<le> 2"
+    by (metis Nat.le_diff_conv2 \<open>line_eq k l\<close> \<open>line_eq l m\<close> add_diff_cancel_right' add_leD2 insert_absorb2 line_eq_refl line_eq_rk rk_couple)
+  then have "rk {fst k, snd k, fst m, snd m} \<le> 2" using matroid_ax_2 by (smt insert_commute order_trans subset_insertI)
+  thus "line_eq k m"
+    using line_eq_def by auto
+qed
 
 lemma ax1_uniqueness : "\<forall>P Q k l. 
 (incid P k) \<longrightarrow> (incid Q k) \<longrightarrow> (incid P l) \<longrightarrow> (incid Q l) \<longrightarrow> (P = Q) \<or> (line_eq k l)"
-
+proof-
+  fix P Q k l
+  assume "incid P k" and "incid Q k" and "incid P l" and "incid Q l"
+  have "line_eq k l" if "P \<noteq> Q"
+  proof-
+    have f1:"rk {P, Q} = 2"
+      by (simp add: rk_couple that)
+    have f2:"rk {fst k, snd k, P, Q} = 2" using matroid_ax_3_alt'
+      by (smt Higher_Proj_Space_Rank_Axioms_To_Higher_Proj_Space_Axioms.fst_def Higher_Proj_Space_Rank_Axioms_To_Higher_Proj_Space_Axioms.snd_def Rep_lines Un_insert_left \<open>incid P k\<close> \<open>incid Q k\<close> incid_rk insert_absorb2 insert_is_Un matroid_ax_2 mem_Collect_eq rk_triple_rep subset_insertI)
+    have f3:"rk {fst l, snd l, P, Q} = 2" using matroid_ax_3_alt'
+      by (smt Un_insert_right \<open>incid P l\<close> \<open>incid Q l\<close> incid_rk insert_absorb2 insert_commute line_eq_refl line_eq_rk sup_bot.right_neutral)
+    have f4:"rk {fst k, snd k, fst l, snd l, P, Q} + rk {P, Q} \<le> rk {fst k, snd k, P, Q} + rk {fst l, snd l, P, Q}"
+      using matroid_ax_3_alt[of "{P, Q}" "{fst k, snd k, P, Q}" "{fst l, snd l, P, Q}"]
+      by (simp add: insert_commute)
+    from f1 and f2 and f3 and f4 have "rk {fst k, snd k, fst l, snd l, P, Q} \<le> 2" by auto
+    thus "line_eq k l" using matroid_ax_2 by (smt eq_iff f3 insert_mono insert_subset line_eq_def)
+  qed
+  show "P = Q \<or> line_eq k l"
 
 
 
